Progress no-error proof

pancake/serial/serialPanDrvProofScript.sml
@@ -1,4 +1,4 @@
-open preamble backendTheory panLangTheory word_to_wordTheory pan_to_wordTheory x64_configTheory compilationLib;
+open preamble backendTheory panLangTheory word_to_wordTheory pan_to_wordTheory;
 open serialPanDrvTheory panSemTheory;
 
 val _ = new_theory "serialPanDrvProof"
@@ -8,7 +8,7 @@ Definition uart_device_oracle_def:
 End
 
 Definition uart_init_state_def:
-  uart_init_state ck be mem memaddrs ffi =
+  uart_init_state ck be mem memaddrs ffi base_addr =
   <| locals := FEMPTY;
      code := FEMPTY |++ serialProg;
      eshapes := FEMPTY; (* TODO: should there be something here? *)
@@ -16,8 +16,9 @@ Definition uart_init_state_def:
      memaddrs := memaddrs;
      clock := ck;
      be := be;
-     ffi := ffi
-    |> 
+     ffi := ffi;
+     base_addr := base_addr
+    |>
 End
 
 Theorem uart_drv_getcharFun_no_break:
@@ -27,9 +28,48 @@ Theorem uart_drv_getcharFun_no_break:
     preconditions (* TODO *) ⇒
     res ≠ SOME Break
 Proof
+  cheat
   (* TODO *)
 QED
-        
+
+Theorem uart_drv_getcharFun_no_error:
+  ∀ck be mem memaddrs ffi base_addr res s.
+    IS_SOME(read_bytearray base_addr 8 (mem_load_byte mem memaddrs be)) ∧
+    more preconditions (* TODO *) ⇒
+    case evaluate (Call Tail (Label (strlit "uart_drv_getchar")) [],
+               uart_init_state ck be mem memaddrs ffi base_addr) of
+      (SOME Error,s') => F
+    | _ => T
+Proof
+  rpt strip_tac >>
+  simp[Once evaluate_def,uart_init_state_def,serialProg_def,
+     uart_drv_getcharFun_def, uart_drv_putcharFun_def] >>
+  simp[Once eval_def,flookup_fupdate_list,ALOOKUP_def,OPT_MMAP_def,lookup_code_def] >>
+  IF_CASES_TAC >- simp[] >>
+  simp[dec_clock_def] >>
+  simp[Once evaluate_def] >>
+  simp[Once eval_def] >>
+  qmatch_goalsub_abbrev_tac ‘a1 (evaluate _)’ >>
+  simp[Once evaluate_def] >>
+  simp[eval_def,OPT_MMAP_def,wordLangTheory.word_op_def] >>
+  qmatch_goalsub_abbrev_tac ‘a2 (evaluate _)’ >>
+  simp[Once evaluate_def,eval_def] >>
+  qmatch_goalsub_abbrev_tac ‘a3 (evaluate _)’ >>
+  simp[Once evaluate_def,eval_def] >>
+  qmatch_goalsub_abbrev_tac ‘a4 (evaluate _)’ >>
+  simp[Once evaluate_def,eval_def] >>
+  qmatch_goalsub_abbrev_tac ‘a5 (evaluate _)’ >>
+  simp[Once evaluate_def,eval_def] >>
+  qmatch_goalsub_abbrev_tac ‘a6 (evaluate _)’ >>
+  simp[Once evaluate_def,FLOOKUP_UPDATE] >>
+  Cases_on ‘read_bytearray base_addr 8 (mem_load_byte mem' memaddrs be)’
+  >- (simp[] >>
+      unabbrev_all_tac >>
+      fs[]) >>
+  simp[] >>
+  cheat (* TODO *)
+QED
+
 Theorem uart_drv_getcharFun_no_error:
   ∀ck be mem memaddrs ffi res s.
     (evaluate (Call Tail (Label (strlit "uart_drv_getchar")) [],
@@ -40,7 +80,8 @@ Proof
   rpt strip_tac >>
   fs[Once evaluate_def,uart_init_state_def,serialProg_def,
      uart_drv_getcharFun_def, uart_drv_putcharFun_def] >>
-  fs[Once eval_def,flookup_fupdate_list,ALOOKUP_def] >>
+  fs[Once eval_def,flookup_fupdate_list,ALOOKUP_def,OPT_MMAP_def,lookup_code_def] >>
+  fs[Once eval_def]
   (* TODO *)
 QED
 
